{
 "cells": [
  {
   "cell_type": "markdown",
   "id": "844f803d-f51e-4d3e-946d-94f88875a4e2",
   "metadata": {},
   "source": [
    "$\\textbf{LESSON 1: ASSIGNMENT ANSWERS}$\n",
    "-"
   ]
  },
  {
   "cell_type": "markdown",
   "id": "34ff3e63-2c97-46f8-a83a-17f07bbbd959",
   "metadata": {},
   "source": [
    "$\\textbf{1. Recall the definition of a rational number, denoted as $\\mathbb{Q}$. Prove that the Euler's number $e = \\Sigma_{k=0}^\\infty \\frac{1}{k!} \\notin \\mathbb{Q}$}$\n",
    "$\\textbf{A factorial is defined as $k! = (k)(k-1)(k-2)(k-3)..., \\forall k \\in \\mathbb{Z}^+$, note that $0! = 1$.}$. \n",
    "$\\textbf{Furthermore, a sum notation $\\Sigma_{k=0}^\\infty k = 0+ 1 + 2 + 3 +....+...$}$}$."
   ]
  },
  {
   "cell_type": "markdown",
   "id": "709b75fb-fca2-49ca-b3b7-c17e742c0580",
   "metadata": {},
   "source": [
    "$\\text{Answer:}$\n",
    "\n",
    "Proof by Contradiction:\n",
    "\n",
    "- Suppose, $e = \\frac{m}{n}$\n",
    "\n",
    "Step 1: \n",
    "\n",
    "\\begin{gather}\n",
    "\\frac{m}{n} = \\Sigma_{k=0}^\\infty \\frac{1}{k!} \\\\\n",
    "n! ( \\frac{m}{n} = \\Sigma_{k=0}^\\infty \\frac{1}{k!} ) n!\\\\\n",
    "\\frac{m}{n}n! = \\Sigma_{k=0}^\\infty \\frac{n!}{k!} \\\\\n",
    "m(n-1)! = \n",
    "\\end{gather}\n",
    "\n",
    "Step 2: Expand\n",
    "\n",
    "\\begin{gather}\n",
    "\\Sigma_{k=0}^\\infty \\frac{n!}{k!} =\n",
    "n! + \\frac{n!}{1!} + \\frac{n!}{2!} + ... + \\frac{n!}{n!} + \\frac{n!}{(n + 1)!} + \\frac{n!}{(n + 2)!} + ...\n",
    "\\end{gather}\n",
    "\n",
    "Step 3: Separate finite set and infinite set\n",
    "\n",
    "\\begin{gather}\n",
    "\\Sigma_{k=0}^n \\frac{n!}{k!} = n! + \\frac{n!}{1!} + \\frac{n!}{2!} + ... + \\frac{n!}{n!} \\\\\n",
    "\\Sigma_{k=n + 1}^\\infty \\frac{n!}{k!} = \\frac{n!}{(n + 1)!} + \\frac{n!}{(n + 2)!} + ...\n",
    "\\end{gather}\n",
    "\n",
    "Step 4: \n",
    "\n",
    "\\begin{gather}\n",
    "m(n - 1)! = \\Sigma_{k=0}^n \\frac{n!}{k!} + \\Sigma_{k=n + 1}^\\infty \\frac{n!}{k!}\n",
    "\\end{gather}\n",
    "\n",
    "- We know that $m(n-1)!$, is an integer, therefore, when we add $\\Sigma_{k=0}^n \\frac{n!}{k!}$ and $\\Sigma_{k=n + 1}^\\infty \\frac{n!}{k!}$, they must result into an integer\n",
    "\n",
    "Step 5: Prove $\\Sigma_{k=0}^n \\frac{n!}{k!}$ is an integer\n",
    "\n",
    "\\begin{gather}\n",
    "\\frac{n!}{k!} = \\frac{n(n-1)(n-2)...k(k-1)(k-2)...}{k(k-1)(k-2)...} = n(n-1)(n-2)...\n",
    "\\end{gather}\n",
    "\n",
    "- Therefore, it is an integer\n",
    "\n",
    "Step 6: Contradiction\n",
    "\n",
    "\\begin{gather}\n",
    "\\Sigma_{k=n + 1}^\\infty \\frac{n!}{k!} = \\frac{n!}{(n + 1)!} + \\frac{n!}{(n + 2)!} + \\frac{n!}{(n + 3)!}\\dotsb \\\\ \n",
    "                                      = \\frac{1}{n+1} + \\frac{1}{(n+1)(n+2)} + \\frac{1}{(n+1)(n+2)(n+3)}\\dotsb\\\\\n",
    "                                      = \\frac{1}{n+1} \\begin{bmatrix} 1+\\frac{1}{n+2}+\\frac{1}{(n+2)(n+3)}+\\dotsb \\end{bmatrix}\\\\\n",
    "                                      < \\frac{1}{n+1} \\begin{bmatrix} 1+\\frac{1}{n+1}+\\frac{1}{(n+1)^2}+\\dotsb \\end{bmatrix} \\text{<--Upper Bound which is 1}\n",
    "\\end{gather}\n",
    "\n",
    "Step 7: Continuation\n",
    "\n",
    "- Remember $S = \\frac{a_0}{1 - 3}$ s.t. $a_0 =$ initial value, $r =$ common ratio\n",
    "- Let $a_0 = \\frac{1}{n+1}$, $r = \\frac{1}{n+1}$\n",
    "- Then:\n",
    "\n",
    "\\begin{gather}\n",
    "S = \\frac{\\frac{1}{n+1}}{1 - \\frac{1}{n+1}}\\\\\n",
    "     = \\frac{1}{n} < 1\n",
    "\\end{gather}\n",
    "\n",
    "- Since, the number should be strictly greater than $0$, then:\n",
    "\\begin{gather}\n",
    "0 < \\frac{1}{n} < 1\n",
    "\\end{gather}\n",
    "\n",
    "- There is no Integer between $0$ and $1$, then that contradicts our supposition. Therefore, $e \\notin \\mathbb{Q}$"
   ]
  },
  {
   "cell_type": "markdown",
   "id": "606eeea7-0ebe-409f-b6f7-97e2d2a52a74",
   "metadata": {},
   "source": [
    "\n",
    "$\\textbf{2. Prove Minkowski's Inequality for sums, $\\forall \\ p>1, (a_k, b_k)>0$:}$\n",
    "\\begin{gather} \n",
    "\\begin{bmatrix} \n",
    "\\Sigma_{k=1}^n |a_k + b_k|^p \n",
    "\\end{bmatrix}^\\frac{1}{p}\n",
    "\\leq\n",
    "\\begin{bmatrix} \n",
    "\\Sigma_{k=1}^n |a_k|^p \n",
    "\\end{bmatrix}^ \\frac{1}{p}\n",
    "+\n",
    "\\begin{bmatrix}\n",
    "\\Sigma_{k=1}^n |b_k|^p\n",
    "\\end{bmatrix}^\\frac{1}{p}\n",
    "\\end{gather}"
   ]
  },
  {
   "cell_type": "markdown",
   "id": "f0e14588-7cbe-44e7-8185-59227c63b7ee",
   "metadata": {},
   "source": [
    "$\\text{Answer:}$\n",
    "\n",
    "Step 1: Laws of Exponents (Power raised to a power):\n",
    "\n",
    "- Let $n = $ any base number, then ${(n^p)}^\\frac{1}{p}=n$\n",
    "- Thus,\n",
    "\\begin{gather} \n",
    "\\Sigma_{k=1}^n |a_k + b_k|\n",
    "\\leq\n",
    "\\Sigma_{k=1}^n |a_k|\n",
    "+\n",
    "\\Sigma_{k=1}^n |b_k|\n",
    "\\end{gather}\n",
    "\n",
    "Step 2: Property of Summation (Addition)\n",
    "\n",
    "\\begin{gather} \n",
    "\\Sigma_{k=1}^n |a_k + b_k|\n",
    "\\leq\n",
    "\\Sigma_{k=1}^n |a_k| + |b_k|\n",
    "\\end{gather}\n",
    "\n",
    "Step 3: Prove by Triangle Inequality\n",
    "\n",
    "- Disregarding the Sigma Notation we get:\n",
    "\\begin{gather}\n",
    "|a_k + b_k|\n",
    "\\leq\n",
    "|a_k| + b_k| \n",
    "\\end{gather}\n",
    "\n",
    "- Since, $(a_k, b_k) > 0$, then $(a + b) = a + b$, and $|a| = a_k$, $|b| = b$:\n",
    "- Substitute:\n",
    "\\begin{gather}\n",
    "|a + b| = a + b = |a| + |b|\n",
    "\\end{gather}"
   ]
  },
  {
   "cell_type": "markdown",
   "id": "fd43a720-cf06-441f-8381-98f154cde0c0",
   "metadata": {},
   "source": [
    "$\\textbf{3. Prove the triangle inequality $|x+y| \\leq |x| + |y|, \\forall (x,y) \\in \\mathbb{R}$}$"
   ]
  },
  {
   "cell_type": "markdown",
   "id": "d3107be2-ece1-4b5b-970c-8aa0b8ff31f3",
   "metadata": {},
   "source": [
    "$\\text{Answer:}$\n",
    "\n",
    "Step 1: Definition of an absolute value\n",
    "\n",
    "- Definition\n",
    "\\begin{gather}\n",
    "{|x| = }\n",
    "\\begin{cases}\n",
    "x,&{x \\geq 0}\\\\ -x,&{x < 0}\n",
    "\\end{cases}\n",
    "\\end{gather}\n",
    "\n",
    "- Thus, we must solve for 4 cases:\n",
    "\n",
    "\\begin{gather}\n",
    "\\text{Case 1: }{x \\geq 0, y \\geq 0} \\\\\n",
    "\\text{Case 2: }{x < 0, y < 0} \\\\\n",
    "\\text{Case 3: }{x \\geq 0, y < 0} \\\\\n",
    "\\text{Case 4: }{x < 0, y \\geq 0} \\\\\n",
    "\\end{gather}\n",
    "\n",
    "Case 1: $x \\geq 0, y \\geq 0$\n",
    "\n",
    "- Let, $|x + y| = x + y$, and $|x| = x, |y| = y$\n",
    "- Substitution:\n",
    "\\begin{gather}\n",
    "|x + y| = x + y = |x| + |y|\n",
    "\\end{gather}\n",
    "\n",
    "Case 2: $x < 0, y < 0$\n",
    "\n",
    "- Let, $|x + y| = -(x + y)$, and $|x| = -x, |y| = -y$\n",
    "- Substitution:\n",
    "\\begin{gather}\n",
    "|x + y| = -(x + y) = -x + (-y) = |x| + |y|\n",
    "\\end{gather}\n",
    "\n",
    "Case 3: $x \\geq 0, y < 0$\n",
    "\n",
    "- Let, $|x| = x, |y| = -y$\n",
    "- Substitution:\n",
    "\\begin{gather}\n",
    "|x + y| \\leq x - y\n",
    "\\end{gather}\n",
    "- Since, $x$ and $y$ are different signs, let's consider two sub-cases for $|x + y|$:\n",
    "\\begin{gather}\n",
    "x + y, x + y \\geq 0 \\\\\n",
    "-(x + y), x + y < 0 \\\\\n",
    "\\end{gather}\n",
    "\n",
    "For $x + y \\geq 0$:\n",
    "\\begin{gather}\n",
    "x + y \\leq x - y \\\\\n",
    "y \\leq -y \n",
    "\\end{gather}\n",
    "\n",
    "For $x + y < 0$:\n",
    "\\begin{gather}\n",
    "-(x + y) \\leq x - y \\\\\n",
    "-x - y \\leq x - y \\\\\n",
    "-x \\leq x \n",
    "\\end{gather}\n",
    "\n",
    "Case 4: $x < 0, y \\geq 0$\n",
    "\n",
    "- Let, $|x| = -x, |y| = y$\n",
    "- Substitution:\n",
    "\\begin{gather}\n",
    "|x + y| \\leq -x + y\n",
    "\\end{gather}\n",
    "- Solve for sub-cases of $|x + y|$:\n",
    "\\begin{gather}\n",
    "x + y, x + y \\geq 0 \\\\\n",
    "-(x + y), x + y < 0 \\\\\n",
    "\\end{gather}\n",
    "\n",
    "For $x + y \\geq 0$:\n",
    "\\begin{gather}\n",
    "x + y \\leq -x + y \\\\\n",
    "x \\leq -x\n",
    "\\end{gather}\n",
    "\n",
    "For $x + y < 0$:\n",
    "\\begin{gather}\n",
    "-(x + y) \\leq -x + y \\\\\n",
    "-x - y \\leq -x + y \\\\\n",
    "-y \\leq y\n",
    "\\end{gather}"
   ]
  },
  {
   "cell_type": "markdown",
   "id": "e817c5b4-05d8-4896-a7ca-a1765174f753",
   "metadata": {},
   "source": [
    "$\\textbf{4. Prove Sedrakayan's Lemma $\\forall u_i, v_i \\in \\mathbb{R}^+$:}$\n",
    "\n",
    "\\begin{gather}\n",
    "\\frac{(\\Sigma_{i=1}^n u_i)^2}{\\Sigma_{i=1}^n v_i}\n",
    "\\leq\n",
    "\\Sigma_{i=1}^n \\frac{(u_i)^2}{v_i}\n",
    "\\end{gather}"
   ]
  },
  {
   "cell_type": "markdown",
   "id": "da2bd635-1de2-485c-aeba-cc9bdde55f82",
   "metadata": {},
   "source": [
    "$\\text{Answer:}$\n",
    "\n",
    "Assume $\\frac{a}{b}\\leq c$, then, $a \\leq cb$\n",
    "\n",
    "Therefore:\n",
    "\n",
    "-\n",
    "\\begin{gather}\n",
    "\\frac{(\\Sigma_{i=1}^n u_i)^2}{\\Sigma_{i=1}^n v_i}\n",
    "\\leq\n",
    "\\Sigma_{i=1}^n \\frac{(u_i)^2}{v_i}\n",
    "\\end{gather}\n",
    "-\n",
    "\\begin{gather}\n",
    "(\\Sigma_{i=1}^n u_i)^2\n",
    "\\leq\n",
    "\\Sigma_{i=1}^n \\frac{(u_i)^2}{v_i} (\\Sigma_{i=1}^n v_i)\n",
    "\\end{gather}"
   ]
  }
 ],
 "metadata": {
  "kernelspec": {
   "display_name": "Python 3 (ipykernel)",
   "language": "python",
   "name": "python3"
  },
  "language_info": {
   "codemirror_mode": {
    "name": "ipython",
    "version": 3
   },
   "file_extension": ".py",
   "mimetype": "text/x-python",
   "name": "python",
   "nbconvert_exporter": "python",
   "pygments_lexer": "ipython3",
   "version": "3.11.4"
  }
 },
 "nbformat": 4,
 "nbformat_minor": 5
}
